theory/x64Semantics.thy
@@ -188,17 +188,22 @@ lemma x64_sem_add:
 type_synonym hybrid_state = "u64 \<times> outcome"
 
 definition one_step:: " (nat \<times> u64 \<times> x64_bin) list \<Rightarrow> hybrid_state\<Rightarrow> hybrid_state" where
-"one_step lt st  \<equiv> let pc = fst st; xst = snd st in 
-  (let (num,off,l) = lt!(unat pc) in
-    (case xst of Next xpc rs m \<Rightarrow> 
+"one_step lt st  \<equiv>
+  let pc = fst st; xst = snd st in 
+  let (num,off,l) = lt!(unat pc) in
+    case xst of
+    Next xpc rs m \<Rightarrow> (
       if off \<noteq> 0 then 
         let xst_temp = Next 0 rs m; xst' = x64_sem num l xst_temp in
-        case xst' of Next xpc' rs' m' \<Rightarrow>
-          if rs' (CR ZF) = 1 then (off+pc, xst')
-          else (pc+1, xst') |
-         Stuck \<Rightarrow> (pc, Stuck)
-      else let xst_temp = Next 0 rs m; xst' = x64_sem num l xst_temp in (pc+1, xst')
-    | Stuck \<Rightarrow> (pc,Stuck)))"
+          case xst' of
+          Next xpc' rs' m' \<Rightarrow>
+            if rs' (CR ZF) = 1 then (off+pc, xst')
+            else (pc+1, xst') |
+          Stuck \<Rightarrow> (pc, Stuck)
+      else
+        let xst_temp = Next 0 rs m; xst' = x64_sem num l xst_temp in
+          (pc+1, xst'))
+    | Stuck \<Rightarrow> (pc,Stuck)"
 
 fun x64_sem1 :: "nat \<Rightarrow> (nat \<times> u64 \<times> x64_bin) list \<Rightarrow> hybrid_state \<Rightarrow> hybrid_state" where
 "x64_sem1 0 _ (pc,st) = (pc,st)" |
