theory/JITPer_mul1.thy
@@ -1,0 +1,275 @@
+theory JITPer_mul1
+imports
+  Main
+  rBPFCommType rBPFSyntax rBPFSem
+  x64Syntax x64Semantics x64Assembler
+  JITPer_aux
+
+begin
+
+lemma mulq_one_step_match_reg:
+  " (SBPF_OK pc' rs' m') = sbpf_step prog (SBPF_OK pc rs m) \<Longrightarrow>
+    xst = (Next xpc xrs xm) \<Longrightarrow>
+    match_state (SBPF_OK pc rs m) (pc,xst) \<Longrightarrow>
+    prog \<noteq> [] \<and> unat pc < length prog \<and> unat pc \<ge> 0 \<Longrightarrow>
+    prog!(unat pc) = BPF_ALU64 BPF_MUL dst (SOReg src) \<Longrightarrow>
+    (bpf_to_x64_reg dst) = RDX \<Longrightarrow>
+      match_reg rs'
+     ((\<lambda>a::preg.
+          if a = IR RDX then xrs (IR RDX) * xrs (IR (bpf_to_x64_reg src))
+          else if a = IR RDX then xrs (IR RDX) * xrs (IR (bpf_to_x64_reg src)) div (4294967296::64 word)
+               else if a = IR RAX then xrs (IR RDX) * xrs (IR (bpf_to_x64_reg src))
+                    else if a = IR RAX then xrs (IR RDX) else if a = IR SP then xrs (IR SP) - u64_of_memory_chunk M64 else if a = IR REG_SCRATCH then xrs (IR (bpf_to_x64_reg src)) else xrs a)
+      (IR SP := xrs (IR SP), IR RAX := xrs (IR RAX)))"
+  apply (simp add: match_state_def match_reg_def eval_alu_def eval_reg_def)
+  by (metis bpf_to_x64_reg_corr reg_r11_consist)
+
+lemma mulq_one_step_match_mem:
+  " (SBPF_OK pc' rs' m') = sbpf_step prog (SBPF_OK pc rs m) \<Longrightarrow>
+    xst = (Next xpc xrs xm) \<Longrightarrow>
+    match_state (SBPF_OK pc rs m) (pc,xst) \<Longrightarrow>
+    prog \<noteq> [] \<and> unat pc < length prog \<and> unat pc \<ge> 0 \<Longrightarrow>
+    prog!(unat pc) = BPF_ALU64 BPF_MUL dst (SOReg src) \<Longrightarrow>
+    (bpf_to_x64_reg dst) = RDX \<Longrightarrow>
+storev M64 xm (Vptr sp_block (xrs (IR SP) - u64_of_memory_chunk M64)) (Vlong (xrs (IR RAX))) = Some m1 \<Longrightarrow>
+    loadv M64 m1 (Vptr sp_block (xrs (IR SP) - u64_of_memory_chunk M64)) = Some (Vlong (xrs (IR RAX))) \<Longrightarrow> match_mem m' m1"
+  apply (simp add: match_state_def match_mem_def eval_alu_def eval_reg_def)
+  using sp_block_def store_load_other by auto
+  
+lemma mulq_one_step_match_stack:
+  " (SBPF_OK pc' rs' m') = sbpf_step prog (SBPF_OK pc rs m) \<Longrightarrow>
+    xst = (Next xpc xrs xm) \<Longrightarrow>
+    match_state (SBPF_OK pc rs m) (pc,xst) \<Longrightarrow>
+    prog \<noteq> [] \<and> unat pc < length prog \<and> unat pc \<ge> 0 \<Longrightarrow>
+    prog!(unat pc) = BPF_ALU64 BPF_MUL dst (SOReg src) \<Longrightarrow>
+    (bpf_to_x64_reg dst) = RDX \<Longrightarrow>
+storev M64 xm (Vptr sp_block (xrs (IR SP) - u64_of_memory_chunk M64)) (Vlong (xrs (IR RAX))) = Some m1 \<Longrightarrow>
+    loadv M64 m1 (Vptr sp_block (xrs (IR SP) - u64_of_memory_chunk M64)) = Some (Vlong (xrs (IR RAX))) \<Longrightarrow>
+    match_stack
+     ((\<lambda>a::preg.
+          if a = IR RDX then xrs (IR RDX) * xrs (IR (bpf_to_x64_reg src))
+          else if a = IR RDX then xrs (IR RDX) * xrs (IR (bpf_to_x64_reg src)) div (4294967296::64 word)
+               else if a = IR RAX then xrs (IR RDX) * xrs (IR (bpf_to_x64_reg src))
+                    else if a = IR RAX then xrs (IR RDX) else if a = IR SP then xrs (IR SP) - u64_of_memory_chunk M64 else if a = IR REG_SCRATCH then xrs (IR (bpf_to_x64_reg src)) else xrs a)
+      (IR SP := xrs (IR SP), IR RAX := xrs (IR RAX)))
+     m1"
+  apply (simp add: match_state_def match_stack_def eval_alu_def eval_reg_def)
+  by (metis sp_block_def store_load_other)
+
+lemma mulq_one_step1:
+assumes a0:"s' = sbpf_step prog s" and
+  a1:"s = (SBPF_OK pc rs m)" and
+  a2:"s' = (SBPF_OK pc' rs' m')" and
+  a3:"xst = (Next xpc xrs xm)" and
+  a4:"match_state s (pc,xst)" and
+  a5:"jitper prog = Some x64_prog" and                      
+  a6:"prog \<noteq> [] \<and> unat pc < length prog \<and> unat pc \<ge> 0" and
+  a8:"prog!(unat pc) = BPF_ALU64 BPF_MUL dst (SOReg src)" and
+  a9:"(bpf_to_x64_reg dst) = RDX "
+shows "\<exists> xst'. x64_sem1 1 x64_prog (pc,xst) = (pc',xst') \<and> 
+  match_state s' (pc',xst')"
+
+  apply simp
+(* 1. as BPF_MUL generates a single list of jited x64 assembly, so we only need one step  *)
+  apply(subgoal_tac "\<exists>xst'::outcome. one_step x64_prog (pc, xst) = (pc', xst') \<and> match_state s' (pc', xst')")
+  subgoal
+    by auto
+  subgoal
+    apply (unfold one_step_def Let_def)
+(* 2. according to the code structure of JITPer, removing the first case statement *)
+    apply(subgoal_tac "x64_prog ! unat (fst (pc, xst)) = the (per_jit_mul_reg64 dst src)")
+     prefer 2
+    subgoal
+      using a5 a6 a8 aux5 per_jit_ins_def by fastforce
+    subgoal
+      apply (subgoal_tac "the (per_jit_mul_reg64 dst src) = (6, 0, x64_encode (Pmovq_rr R11 (bpf_to_x64_reg src))@(x64_encode (Ppushl_r RAX)) @ (x64_encode (Pmovq_rr RAX RDX)) 
+                  @ (x64_encode (Pmulq_r R11))@ (x64_encode (Pmovq_rr RDX RAX))@ (x64_encode (Ppopl RAX)))")
+       prefer 2
+      subgoal using per_jit_mul_reg64_def a9 by simp
+      subgoal
+        unfolding a3
+        apply simp
+        apply (erule subst)
+        apply (erule subst)
+(* 3. here we get a simplified version, next step is to run the 6 x64 assembly one by one *)
+(* 3.1 *)
+        apply (subgoal_tac "Suc 5 = (6::nat)") prefer 2 subgoal by simp
+        apply (erule subst)
+        apply (simp only: x64_sem.simps)
+        apply simp
+(* 3.1.1 using consistency to get x64 assembly *)
+        apply (subgoal_tac "x64_decode (0::nat)
+            (x64_encode (Pmovq_rr REG_SCRATCH (bpf_to_x64_reg src)) @
+             x64_encode (Ppushl_r RAX) @ x64_encode (Pmovq_rr RAX RDX) @ x64_encode (Pmulq_r REG_SCRATCH) @ x64_encode (Pmovq_rr RDX RAX) @ x64_encode (Ppopl RAX))
+            = Some (3, Pmovq_rr REG_SCRATCH (bpf_to_x64_reg src))")
+         prefer 2
+        subgoal
+          apply (rule_tac l_bin = "x64_encode (Pmovq_rr REG_SCRATCH (bpf_to_x64_reg src))" in x64_encode_decode_consistency)
+          subgoal using list_in_list_prop
+            using list_in_list_concat by blast
+          subgoal by simp
+          subgoal using x64_encode_def
+            by fastforce
+          done
+        apply simp
+        apply (erule subst)
+        apply (simp add: exec_instr_def)
+(* 3.2 *)
+        apply (subgoal_tac "Suc 4 = (5::nat)") prefer 2 subgoal by simp
+        apply (erule subst)
+        apply (simp only: x64_sem.simps)
+        apply simp
+        apply (subgoal_tac "x64_decode (3::nat)
+            (x64_encode (Pmovq_rr REG_SCRATCH (bpf_to_x64_reg src)) @
+             x64_encode (Ppushl_r RAX) @ x64_encode (Pmovq_rr RAX RDX) @ x64_encode (Pmulq_r REG_SCRATCH) @ x64_encode (Pmovq_rr RDX RAX) @ x64_encode (Ppopl RAX))
+            = Some (1, Ppushl_r RAX)")
+         prefer 2
+(* this is necessary for later list_in_list_prop_aux2 *)
+        apply (subgoal_tac "length (x64_encode (Pmovq_rr REG_SCRATCH (bpf_to_x64_reg src))) = 3")
+         prefer 2 subgoal using x64_encode_def by simp
+        subgoal
+          apply (rule_tac l_bin = "x64_encode (Ppushl_r RAX)" in x64_encode_decode_consistency)
+          subgoal using list_in_list_prop_aux2
+            by metis 
+          subgoal by simp
+          subgoal apply (erule subst) 
+            using x64_encode_def construct_rex_to_u8_def bitfield_insert_u8_def Let_def
+            by fastforce
+          done
+        apply simp
+        apply (erule subst)
+        apply (simp add: exec_instr_def exec_push_def Let_def)
+        apply (insert storev_stack_some [of xm "(xrs (IR SP) - u64_of_memory_chunk M64)" "xrs (IR RAX)"])
+        apply (erule exE)
+        subgoal for m1
+          apply simp
+(* 3.3 *)
+        apply (subgoal_tac "Suc 3 = (4::nat)") prefer 2 subgoal by simp
+        apply (erule_tac subst [of _ 4])
+        apply (simp only: x64_sem.simps)
+        apply simp
+(* using consistency to get x64 assembly *)
+        apply (subgoal_tac "x64_decode (4::nat)
+            (x64_encode (Pmovq_rr REG_SCRATCH (bpf_to_x64_reg src)) @
+             x64_encode (Ppushl_r RAX) @ x64_encode (Pmovq_rr RAX RDX) @ x64_encode (Pmulq_r REG_SCRATCH) @ x64_encode (Pmovq_rr RDX RAX) @ x64_encode (Ppopl RAX))
+            = Some (3, Pmovq_rr RAX RDX)")
+         prefer 2
+(* this is necessary for later list_in_list_prop_aux2 *)
+        apply (subgoal_tac "length ((x64_encode (Pmovq_rr REG_SCRATCH (bpf_to_x64_reg src)) @
+             x64_encode (Ppushl_r RAX))) = 4")
+         prefer 2 subgoal using x64_encode_def construct_rex_to_u8_def bitfield_insert_u8_def Let_def by simp
+        subgoal
+          apply (rule_tac l_bin = "x64_encode (Pmovq_rr RAX RDX)" in x64_encode_decode_consistency)
+          subgoal using list_in_list_prop_aux2
+            by (metis append_assoc)
+          subgoal by simp
+          subgoal using x64_encode_def
+            by fastforce
+          done
+        apply simp
+        apply (erule subst [of _ "Some (3::nat, Pmovq_rr RAX RDX)"])
+        apply (simp add: exec_instr_def)
+(* 3.4 *)
+        apply (subgoal_tac "Suc 2 = (3::nat)") prefer 2 subgoal by simp
+        apply (erule_tac subst [of _ 3])
+        apply (simp only: x64_sem.simps)
+        apply simp
+(* using consistency to get x64 assembly *)
+        apply (subgoal_tac "x64_decode (7::nat)
+            (x64_encode (Pmovq_rr REG_SCRATCH (bpf_to_x64_reg src)) @
+             x64_encode (Ppushl_r RAX) @ x64_encode (Pmovq_rr RAX RDX) @ x64_encode (Pmulq_r REG_SCRATCH) @ x64_encode (Pmovq_rr RDX RAX) @ x64_encode (Ppopl RAX))
+            = Some (3, Pmulq_r REG_SCRATCH)")
+         prefer 2
+(* this is necessary for later list_in_list_prop_aux2 *)
+        apply (subgoal_tac "length ((x64_encode (Pmovq_rr REG_SCRATCH (bpf_to_x64_reg src)) @
+             x64_encode (Ppushl_r RAX) @ x64_encode (Pmovq_rr RAX RDX))) = 7")
+         prefer 2 subgoal using x64_encode_def construct_rex_to_u8_def bitfield_insert_u8_def Let_def by simp
+        subgoal
+          apply (rule_tac l_bin = "x64_encode (Pmulq_r REG_SCRATCH)" in x64_encode_decode_consistency)
+          subgoal using list_in_list_prop_aux2
+            by (metis append_assoc)
+          subgoal by simp
+          subgoal using x64_encode_def
+            by fastforce
+          done
+        apply simp
+        apply (erule subst [of _ "Some (3::nat, Pmulq_r REG_SCRATCH)"])
+        apply (simp add: exec_instr_def)
+(* 3.5 *)
+        apply (subgoal_tac "Suc 1 = (2::nat)") prefer 2 subgoal by simp
+        apply (erule_tac subst [of _ 2])
+        apply (simp only: x64_sem.simps)
+        apply simp
+(* using consistency to get x64 assembly *)
+        apply (subgoal_tac "x64_decode (10::nat)
+            (x64_encode (Pmovq_rr REG_SCRATCH (bpf_to_x64_reg src)) @
+             x64_encode (Ppushl_r RAX) @ x64_encode (Pmovq_rr RAX RDX) @ x64_encode (Pmulq_r REG_SCRATCH) @ x64_encode (Pmovq_rr RDX RAX) @ x64_encode (Ppopl RAX))
+            = Some (3, Pmovq_rr RDX RAX)")
+         prefer 2
+(* this is necessary for later list_in_list_prop_aux2 *)
+        apply (subgoal_tac "length ((x64_encode (Pmovq_rr REG_SCRATCH (bpf_to_x64_reg src)) @
+             x64_encode (Ppushl_r RAX) @ x64_encode (Pmovq_rr RAX RDX))@ x64_encode (Pmulq_r REG_SCRATCH)) = 10")
+         prefer 2 subgoal using x64_encode_def construct_rex_to_u8_def bitfield_insert_u8_def Let_def by simp
+        subgoal
+          apply (rule_tac l_bin = "x64_encode (Pmovq_rr RDX RAX)" in x64_encode_decode_consistency)
+          subgoal using list_in_list_prop_aux2
+            by (metis append_assoc)
+          subgoal by simp
+          subgoal using x64_encode_def
+            by fastforce
+          done
+        apply simp
+        apply (erule subst [of _ "Some (3::nat, Pmovq_rr RDX RAX) "])
+        apply (simp add: exec_instr_def)
+(* 3.6 *)
+        apply (subgoal_tac "Suc 0 = (1::nat)") prefer 2 subgoal by simp
+        apply (erule_tac subst [of _ 1])
+        apply (simp only: x64_sem.simps)
+(* using consistency to get x64 assembly *)
+        apply (subgoal_tac "x64_decode (13::nat)
+            (x64_encode (Pmovq_rr REG_SCRATCH (bpf_to_x64_reg src)) @
+             x64_encode (Ppushl_r RAX) @ x64_encode (Pmovq_rr RAX RDX) @ x64_encode (Pmulq_r REG_SCRATCH) @ x64_encode (Pmovq_rr RDX RAX) @ x64_encode (Ppopl RAX))
+            = Some (1, Ppopl RAX)")
+         prefer 2
+(* this is necessary for later list_in_list_prop_aux2 *)
+        apply (subgoal_tac "length ((x64_encode (Pmovq_rr REG_SCRATCH (bpf_to_x64_reg src)) @
+             x64_encode (Ppushl_r RAX) @ x64_encode (Pmovq_rr RAX RDX))@ x64_encode (Pmulq_r REG_SCRATCH) @ x64_encode (Pmovq_rr RDX RAX)) = 13")
+         prefer 2 subgoal using x64_encode_def construct_rex_to_u8_def bitfield_insert_u8_def Let_def by simp
+        subgoal
+          apply (rule_tac l_bin = "x64_encode (Ppopl RAX)" in x64_encode_decode_consistency)
+          subgoal using list_in_list_prop_aux2
+            by (metis append_eq_append_conv2)
+          subgoal by simp
+          subgoal using x64_encode_def construct_rex_to_u8_def bitfield_insert_u8_def Let_def
+            by fastforce
+          done
+        apply simp
+        apply (erule subst [of _ "Some (Suc (0::nat), Ppopl RAX)"])
+        apply (simp add: exec_instr_def exec_pop_def)
+        apply (frule store_load_consistency)
+        apply simp
+
+(* 4. now we get exec_instr (one step of x64 add assembly), we prove the \<and>, first left, then right *)
+        apply (rule conjI)
+        subgoal
+          by (metis a0 a1 a2 a5 a6 a8 corr_pc_aux2 insert_iff prod_cases3)
+
+        unfolding a1 a2
+        apply (simp add: match_state_def)
+        apply (rule conjI)
+(* 4.1  match_reg *)
+        subgoal using mulq_one_step_match_reg a0 a1 a2 a3 a4 a6 a8 a9
+          by simp
+
+        apply (rule conjI)
+(* 4.2  match_mem *)
+        subgoal using mulq_one_step_match_mem a0 a1 a2 a3 a4 a6 a8 a9 by simp
+(* 4.2  match_stack *)
+        subgoal using mulq_one_step_match_stack a0 a1 a2 a3 a4 a6 a8 a9 by simp
+        done
+      done
+    done
+  done
+  done
+
+end
